TabularTypeInterpreter/Data/Nat.lean
@@ -1,0 +1,32 @@
+namespace Nat
+
+theorem max_eq_or (a b : Nat) : max a b = a ∨ max a b = b := by
+  rw [Max.max, instMax, maxOfLe]
+  simp
+  by_cases a ≤ b
+  · case pos le =>
+    right
+    intro lt
+    nomatch Nat.not_le_of_lt lt le
+  · case neg lt =>
+    left
+    intro le
+    nomatch lt le
+
+theorem max_le_iff (a b c : Nat) : max b c ≤ a ↔ b ≤ a ∧ c ≤ a where
+  mp maxle := by
+    rw [Max.max, instMax, maxOfLe] at maxle
+    simp at maxle
+    split at maxle
+    · case isTrue blec => exact ⟨trans blec maxle, maxle⟩
+    · case isFalse cltb =>
+      exact ⟨maxle, Nat.le_of_lt (Nat.lt_of_lt_of_le (Nat.lt_of_not_le cltb) maxle)⟩
+  mpr
+    | ⟨blea, clea⟩ => by
+      rw [Max.max, instMax, maxOfLe]
+      simp
+      split
+      · case isTrue _ => exact clea
+      · case isFalse _ => exact blea
+
+end Nat
