TabularTypeInterpreter/Data/Option.lean
@@ -1,0 +1,8 @@
+namespace Option
+
+theorem lt_getD [LT α] (lty : ∀ y, y? = some y → x < y) (ltz : y? = none → x < z)
+  : x < Option.getD (α := α) y? z := match y? with
+  | some y => lty y rfl
+  | none => ltz rfl
+
+end Option
